EthCryptographySpecs/Proofs/Kzg.lean
@@ -1,5 +1,6 @@
 import EthCryptographySpecs.Proofs.Kzg.BitReversal
 import EthCryptographySpecs.Proofs.Kzg.Fft
+import EthCryptographySpecs.Proofs.Kzg.Polynomials
 
 /-!
 # `EthCryptographySpecs.Proofs.Kzg`
